BUpdLaws

src/Iris/BI/Updates.lean
@@ -5,21 +5,28 @@ Authors: Markus de Medeiros
 -/
 
 import Iris.BI.BI
+import Iris.BI.BIBase
+import Iris.BI.Classes
+import Iris.BI.DerivedLaws
+import Iris.Algebra
 
 --TODO: Which type should we use for sets of masks?
 abbrev Set (α : Type _) := α → Prop
 abbrev setT {α : Type _} : Set α := fun _ => True
+abbrev subset (x y : Set α) : Prop := ∀ a, x a → y a
 
 class BUpd (PROP : Type _) where
   bupd : PROP → PROP
 export BUpd (bupd)
 
-syntax "|==> " term : term
-syntax term " ==∗ " term : term
+syntax "|==> " term:40 : term
+syntax term:26 " ==∗ " term:25 : term
+
+open Iris BI
 
 macro_rules
-  | `(iprop(|==> $P))  => ``(iprop(bupd $P))
-  | `(iprop($P ==∗ $Q))  => ``(iprop($P -∗ bupd $Q))
+  | `(iprop(|==> $P))  => ``(BUpd.bupd iprop($P))
+  | `(iprop($P ==∗ $Q))  => ``(BIBase.wand iprop($P) (BUpd.bupd iprop($Q)))
 
 delab_rule BUpd.bupd
   | `($_ $P) => do ``(iprop(|==> $(← Iris.BI.unpackIprop P)))
@@ -36,10 +43,10 @@ syntax "|={ " term " }=> " term : term
 syntax term "={ " term " }=∗ " term : term
 
 macro_rules
-  | `(iprop(|={ $E1 , $E2 }=> $P))  => ``(iprop(fupd $E1 $E2 $P))
-  | `(iprop($P ={ $E1 , $E2 }=∗ $Q))  => ``(iprop($P -∗ fupd $E1 $E2 $Q))
-  | `(iprop(|={ $E1 }=> $P))  => ``(iprop(fupd $E1 $P))
-  | `(iprop($P ={ $E1 }=∗ $Q))  => ``(iprop($P -∗ fupd $E1 $Q))
+  | `(iprop(|={ $E1 , $E2 }=> $P))  => ``(FUpd.fupd $E1 $E2 iprop($P))
+  | `(iprop($P ={ $E1 , $E2 }=∗ $Q))  => ``(BIBase.wand iprop($P) (FUpd.fupd $E1 $E2 iprop($Q)))
+  | `(iprop(|={ $E1 }=> $P))  => ``(FUpd.fupd $E1 $E1 iprop($P))
+  | `(iprop($P ={ $E1 }=∗ $Q))  => ``(BIBase.wand iprop($P) (FUpd.fupd $E1 $E1 iprop($Q)))
 
 -- Delab rules
 
@@ -50,13 +57,12 @@ syntax "|={ " term " }▷=> " term : term
 syntax term "={ " term " }▷=∗ " term : term
 
 macro_rules
-  | `(iprop(|={ $E1 }[ $E2 ]▷=> $P))  => ``(iprop(|={$E1, $E2}=> ▷ (|={ $E2, $E1 }=> $P)))
-  | `(iprop($P ={ $E1 }[ $E2 ]▷=∗ $Q))  => ``(iprop($P -∗ |={$E1}[$E2]▷=> $Q))
-  | `(iprop(|={ $E1 }▷=> $P))  => ``(iprop(|={$E1}[$E1]▷=> $P))
-  | `(iprop($P ={ $E1 }▷=∗ $Q))  => ``(iprop($P ={$E1}[$E1]▷=∗ $Q))
+  | `(iprop(|={ $E1 }[ $E2 ]▷=> $P))  => ``(iprop(|={$E1, $E2}=> ▷ (|={ $E2, $E1 }=> iprop($P))))
+  | `(iprop($P ={ $E1 }[ $E2 ]▷=∗ $Q))  => ``(iprop(iprop($P) -∗ |={$E1}[$E2]▷=> iprop($Q)))
+  | `(iprop(|={ $E1 }▷=> $P))  => ``(iprop(|={$E1}[$E1]▷=> iprop($P)))
+  | `(iprop($P ={ $E1 }▷=∗ $Q))  => ``(iprop(iprop($P) ={$E1}[$E1]▷=∗ iprop($Q)))
 
 -- Delab rules
-
 
 syntax "|={ " term " }[ " term " ]▷^" term "=> " term : term
 syntax term "={ " term " }[ " term " ]▷^" term "=∗ " term : term
@@ -64,21 +70,82 @@ syntax "|={ " term " }▷^" term "=> " term : term
 syntax term "={ " term " }▷^" term "=∗ " term : term
 
 macro_rules
-  | `(iprop(|={ $E1 }[ $E2 ]▷^$n=> $P))  => ``(iprop(|={$E1, $E2}=> ▷^[$n] (|={ $E2, $E1 }=> $P)))
-  | `(iprop($P ={ $E1 }[ $E2 ]▷^$n=∗ $Q))  => ``(iprop($P -∗ |={$E1}[$E2]▷^$n=> $Q))
-  | `(iprop(|={ $E1 }▷^$n=> $P))  => ``(iprop(|={$E1}[$E1]▷^$n=> $P))
-  | `(iprop($P ={ $E1 }▷^$n=∗ $Q))  => ``(iprop($P ={$E1}[$E1]▷^$n=∗ $Q))
+  | `(iprop(|={ $E1 }[ $E2 ]▷^$n=> $P))  => ``(iprop(|={$E1, $E2}=> ▷^[$n] (|={ $E2, $E1 }=> iprop($P))))
+  | `(iprop($P ={ $E1 }[ $E2 ]▷^$n=∗ $Q))  => ``(iprop(iprop($P) -∗ |={$E1}[$E2]▷^$n=> iprop($Q)))
+  | `(iprop(|={ $E1 }▷^$n=> $P))  => ``(iprop(|={$E1}[$E1]▷^$n=> iprop($P)))
+  | `(iprop($P ={ $E1 }▷^$n=∗ $Q))  => ``(iprop(iprop($P) ={$E1}[$E1]▷^$n=∗ iprop($Q)))
 
 -- Delab rules
 
 namespace Iris.BI
 open Iris.Std BI
 
+class BiUpdate (PROP : Type _) [BI PROP] extends BUpd PROP where
+  [bupd_nonexpansive : OFE.NonExpansive (BUpd.bupd (PROP := PROP))]
+  intro {P : PROP} : iprop(P ⊢ |==> P)
+  mono {P Q : PROP} : iprop(P ⊢ Q) → iprop(|==> P ⊢ |==> Q)
+  trans {P : PROP} : iprop(|==> |==> P ⊢ |==> P)
+  frame_r {P R : PROP} : iprop((|==> P) ∗ R ⊢ |==> (P ∗ R))
+
+class BiFUpdate (PROP MASK : Type _) [BI PROP] extends FUpd PROP MASK where
+  [nonexpansive {E1 E2 : Set MASK} : OFE.NonExpansive (FUpd.fupd E1 E2 (PROP := PROP))]
+  subset {E1 E2 : Set MASK} :
+    subset E2 E1 → iprop(⊢ |={E1, E2}=> |={E2, E1}=> (emp : PROP))
+  except0 {E1 E2 : Set MASK} (P : PROP) :
+    iprop((◇ |={E1, E2}=> P) ⊢ |={E1, E2}=> P)
+  trans {E1 E2 E3 : Set MASK} (P : PROP) :
+    iprop((|={E1, E2}=> |={E2, E3}=> P) ⊢ |={E1, E3}=> P)
+  -- What is the reason for frame_r'?
+  frame_r {E1 E2 : Set MASK} (P R : PROP) :
+    iprop((|={E1, E2}=> P) ∗ R ⊢ |={E1, E2}=> P ∗ R)
+
+class BiUpdateFUpdate (PROP : Type _) [BI PROP] [BiUpdate PROP] [BiFUpdate PROP MASK] where
+  fupd_of_bupd (P : PROP) (E : Set MASK) : iprop(⊢ |==> P) → iprop(⊢ |={E}=> P)
+
+-- TODO: Plainly updates
+
+section BUpdLaws
+
+variable {PROP : Type _} [BI PROP] [BiUpdate PROP]
+
+open BI BiUpdate
+
+theorem frame_l {P Q : PROP} : iprop(P ∗ |==> Q ⊢ |==> (P ∗ Q)) :=
+  sep_symm.trans <| frame_r.trans <| mono <| sep_symm
+
+theorem wand_l {P Q : PROP} : iprop((P -∗ Q) ∗ (|==> P) ⊢ |==> Q) :=
+  frame_l.trans <| mono <| wand_elim <| .rfl
+
+theorem wand_r {P Q : PROP} : iprop((|==> P) ∗ (P -∗ Q) ⊢ |==> Q) :=
+  sep_symm.trans wand_l
+
+theorem bupd_sep {P Q : PROP} : iprop((|==> P) ∗ (|==> Q) ⊢ |==> (P ∗ Q)) :=
+  frame_l.trans <| (mono <| frame_r).trans <| BiUpdate.trans
+
+theorem idemp {P : PROP} : iprop((|==> |==> P) ⊣⊢ |==> P) :=
+  ⟨BiUpdate.trans, BiUpdate.intro⟩
+
+theorem bupd_or {P Q: PROP} : iprop((|==> P) ∨ (|==> Q) ⊢ |==> (P ∨ Q)) :=
+  or_elim (mono or_intro_l) (mono or_intro_r)
+
+theorem bupd_and {P Q : PROP} : iprop((|==> (P ∧ Q)) ⊢ (|==> P) ∧ (|==> Q)) :=
+  and_intro (mono and_elim_l) (mono and_elim_r)
+
+-- Exist and Forall
+-- Big ops
+
+theorem bupd_except_0 {P : PROP} : iprop(◇ (|==> P) ⊢ (|==> ◇ P)) :=
+  or_elim (or_intro_l.trans intro) (mono or_intro_r)
+
+instance {P : PROP} [Absorbing P] : Absorbing iprop(|==> P) :=
+  ⟨frame_l.trans <| mono <| sep_elim_r⟩
+
+end BUpdLaws
 
 
--- example [BI PROP] [BUpd PROP] (P Q : PROP) : ⊢ iprop(R ∗ P) := sorry
-example [BI PROP] [BUpd PROP] (P : PROP) : ⊢ iprop(|==> P) := sorry
--- example [BI PROP] [BUpd PROP] (P : PROP) : ⊢ iprop(|==> P ∗ P) := sorry
-example [BI PROP] [BUpd PROP] (P Q : PROP) : ⊢ iprop(R ∗ P ==∗ Q) := sorry
--- example [BI PROP] [BUpd PROP] (P Q R : PROP) : ⊢ iprop(R ∗ P ==∗ Q -∗ R) := sorry
-example [BI PROP] [BUpd PROP] (P Q : PROP) : ⊢ iprop(P -∗ |==> P) := sorry
+-- -- example [BI PROP] [BUpd PROP] (P Q : PROP) : ⊢ iprop(R ∗ P) := sorry
+-- example [BI PROP] [BUpd PROP] (P : PROP) : ⊢ iprop(|==> P) := sorry
+-- -- example [BI PROP] [BUpd PROP] (P : PROP) : ⊢ iprop(|==> P ∗ P) := sorry
+-- example [BI PROP] [BUpd PROP] (P Q : PROP) : ⊢ iprop(R ∗ P ==∗ Q) := sorry
+-- -- example [BI PROP] [BUpd PROP] (P Q R : PROP) : ⊢ iprop(R ∗ P ==∗ Q -∗ R) := sorry
+-- example [BI PROP] [BUpd PROP] (P Q : PROP) : ⊢ iprop(P -∗ |==> P) := sorry
